[CFG] Prove soundness of rules for a sequential block

Hoare/HoareCFG.thy
@@ -314,4 +314,84 @@ lemma triple_inst_soundness:
   apply(simp add: inst_false_pre_sem)
 done
 
+(* Define the semantic of triple_seq and prove it sound *)
+
+definition triple_seq_sem :: "pred \<Rightarrow> pos_inst list \<Rightarrow> pred \<Rightarrow> bool" where
+"triple_seq_sem pre insts post ==
+    \<forall>co_ctx presult rest stopper net.
+			no_assertion co_ctx \<longrightarrow>
+      (pre ** code (set insts) ** rest) (instruction_result_as_set co_ctx presult) \<longrightarrow>
+      ((post ** code (set insts) ** rest) (instruction_result_as_set co_ctx (program_sem stopper co_ctx (length insts) net presult)))"
+
+lemma inst_seq_eq:
+"triple_inst P i Q \<Longrightarrow> triple_seq_sem P [i] Q"
+ apply(drule triple_inst_soundness)
+ apply(simp add: triple_inst_sem_def triple_seq_sem_def)
+ apply(fastforce)
+done
+
+lemma seq_compose_soundness:
+notes sep_fun_simps[simp del]
+shows
+"triple_seq_sem P xs R \<Longrightarrow> triple_seq_sem R ys Q \<Longrightarrow> triple_seq_sem P (xs@ys) Q "
+ apply(simp (no_asm) add: triple_seq_sem_def)
+ apply clarsimp
+ apply(subst (asm) triple_seq_sem_def[where pre=P])
+ apply clarsimp
+ apply(rename_tac co_ctx presult rest stopper net)
+ apply(drule_tac x = "co_ctx" in spec, simp)
+ apply(drule_tac x = "presult" in spec)
+ apply(drule_tac x = "code ((set ys) - (set xs)) ** rest" in spec)
+ apply(simp add: code_more sep_conj_ac)
+ apply(drule_tac x = stopper in spec)
+ apply(drule_tac x = "net" in spec)
+ apply(clarsimp simp add: triple_seq_sem_def)
+ apply(drule_tac x = "co_ctx" in spec; simp)
+ apply(drule_tac x = "program_sem stopper co_ctx (length xs) net presult" in spec)
+ apply(drule_tac x = "code ((set xs) - (set ys)) ** rest" in spec)
+ apply(simp add: code_more sep_conj_ac code_union_comm)
+ apply(drule_tac x = stopper in spec)
+ apply(drule_tac x = "net" in spec)
+ apply(simp add: execution_continue)
+done
+
+lemma triple_seq_empty:
+"(\<And>s. pre s \<longrightarrow> post s) \<Longrightarrow> triple_seq_sem pre [] post"
+ apply (simp add: triple_seq_sem_def program_sem.simps imp_sepL)
+ apply(clarify)
+ apply(drule allI)
+ apply(simp add: imp_sepL)
+done
+
+lemma seq_strengthen_pre_sem:
+  assumes  "triple_seq_sem P c Q"
+  and      "(\<forall> s. R s \<longrightarrow> P s)"
+  shows    " triple_seq_sem R c Q"
+  using assms(1)
+  apply (simp add: triple_seq_sem_def)
+  apply(clarify)
+  apply(drule_tac x = co_ctx in spec)
+  apply(simp)
+  apply(drule_tac x = presult in spec)
+  apply(drule_tac x = rest in spec)
+  apply simp
+  apply(erule impE)
+   apply(sep_drule assms(2)[rule_format])
+   apply assumption
+  apply simp
+done
+
+lemma triple_seq_soundness:
+"triple_seq P xs Q \<Longrightarrow> triple_seq_sem P xs Q"
+ apply(induction rule: triple_seq.induct)
+    apply(drule inst_seq_eq)
+    apply(rename_tac pre x q xs post)
+    apply(subgoal_tac "x#xs = [x]@xs")
+     apply(simp only: seq_compose_soundness)
+    apply(simp)
+   apply(simp add: triple_seq_empty)
+  apply(simp add: seq_strengthen_pre_sem)
+ apply(simp add: triple_seq_sem_def)
+done
+
 end
